More work in parameterized soundness and completeness.

SeparationLogic/Downwards2Upwards.v
@@ -49,7 +49,7 @@ Proof.
       reflexivity.
 Defined.
 
-Definition UsSM {L: Language} {nL: NormalLanguage L} {pL: PropositionalLanguage L} {SL: SeparationLanguage L} {uSL: UnitarySeparationLanguage L} {MD: Model} {kMD: KripkeModel MD} (M: Kmodel) {kiM: KripkeIntuitionisticModel (Kworlds M)} {J: Join (Kworlds M)} {SA: SeparationAlgebra (Kworlds M)} {dSA: DownwardsClosedSeparationAlgebra (Kworlds M)} {USA: UnitarySeparationAlgebra (Kworlds M)} {SM: Semantics L MD} {kiSM: KripkeIntuitionisticSemantics L MD M SM} {dsSM: DownwardsSemantics L MD M SM} {UsSM: UnitarySemantics L MD M SM} : @UnitarySemantics L _ _ _ _ MD _ M kiM (UpwardsClosure_SA) (UpwardsClosure_USA) SM kiSM.
+Definition UsSM {L: Language} {nL: NormalLanguage L} {pL: PropositionalLanguage L} {SL: SeparationLanguage L} {uSL: UnitarySeparationLanguage L} {MD: Model} {kMD: KripkeModel MD} (M: Kmodel) {kiM: KripkeIntuitionisticModel (Kworlds M)} {J: Join (Kworlds M)} {SA: SeparationAlgebra (Kworlds M)} {dSA: DownwardsClosedSeparationAlgebra (Kworlds M)} {USA: UnitarySeparationAlgebra (Kworlds M)} {SM: Semantics L MD} {kiSM: KripkeIntuitionisticSemantics L MD M SM} {dsSM: DownwardsSemantics L MD M SM} {UsSM: UnitarySemantics L MD M SM} : @UnitarySemantics L _ _ _ _ MD _ M kiM (UpwardsClosure_SA) SM kiSM.
 Proof.
   intros m; simpl.
   rewrite <- UpwardsClosure_pre_unit.
@@ -91,7 +91,7 @@ Proof.
       reflexivity.
 Defined.
 
-Definition UsSM {L: Language} {nL: NormalLanguage L} {pL: PropositionalLanguage L} {SL: SeparationLanguage L} {uSL: UnitarySeparationLanguage L} {MD: Model} {kMD: KripkeModel MD} (M: Kmodel) {kiM: KripkeIntuitionisticModel (Kworlds M)} {J: Join (Kworlds M)} {SA: SeparationAlgebra (Kworlds M)} {dSA: DownwardsClosedSeparationAlgebra (Kworlds M)} {USA: UnitarySeparationAlgebra (Kworlds M)} {SM: Semantics L MD} {kiSM: KripkeIntuitionisticSemantics L MD M SM} {dsSM: DownwardsSemantics L MD M SM} {UsSM: UnitarySemantics L MD M SM} : @UnitarySemantics L _ _ _ _ MD _ M kiM (UpwardsClosure_SA) (UpwardsClosure_USA) SM kiSM.
+Definition UsSM {L: Language} {nL: NormalLanguage L} {pL: PropositionalLanguage L} {SL: SeparationLanguage L} {uSL: UnitarySeparationLanguage L} {MD: Model} {kMD: KripkeModel MD} (M: Kmodel) {kiM: KripkeIntuitionisticModel (Kworlds M)} {J: Join (Kworlds M)} {SA: SeparationAlgebra (Kworlds M)} {dSA: DownwardsClosedSeparationAlgebra (Kworlds M)} {USA: UnitarySeparationAlgebra (Kworlds M)} {SM: Semantics L MD} {kiSM: KripkeIntuitionisticSemantics L MD M SM} {dsSM: DownwardsSemantics L MD M SM} {UsSM: UnitarySemantics L MD M SM} : @UnitarySemantics L _ _ _ _ MD _ M kiM (UpwardsClosure_SA) SM kiSM.
 Proof.
   intros m; simpl.
   rewrite <- UpwardsClosure_pre_unit.
