SeparationLogic/Upwards2Downwards.v
@@ -49,7 +49,7 @@ Proof.
         reflexivity.
 Defined.
 
-Definition UsSM {L: Language} {nL: NormalLanguage L} {pL: PropositionalLanguage L} {SL: SeparationLanguage L} {uSL: UnitarySeparationLanguage L} {MD: Model} {kMD: KripkeModel MD} (M: Kmodel) {kiM: KripkeIntuitionisticModel (Kworlds M)} {J: Join  (Kworlds M)} {SA: SeparationAlgebra (Kworlds M)} {uSA: UpwardsClosedSeparationAlgebra (Kworlds M)} {USA: UnitarySeparationAlgebra (Kworlds M)} {SM: Semantics L MD} {kiSM: KripkeIntuitionisticSemantics L MD M SM} {usSM: UpwardsSemantics L MD M SM} {UsSM: UnitarySemantics L MD M SM} : @UnitarySemantics L _ _ _ _ MD _ M kiM (DownwardsClosure_SA ) (DownwardsClosure_USA) SM kiSM.
+Definition UsSM {L: Language} {nL: NormalLanguage L} {pL: PropositionalLanguage L} {SL: SeparationLanguage L} {uSL: UnitarySeparationLanguage L} {MD: Model} {kMD: KripkeModel MD} (M: Kmodel) {kiM: KripkeIntuitionisticModel (Kworlds M)} {J: Join  (Kworlds M)} {SA: SeparationAlgebra (Kworlds M)} {uSA: UpwardsClosedSeparationAlgebra (Kworlds M)} {USA: UnitarySeparationAlgebra (Kworlds M)} {SM: Semantics L MD} {kiSM: KripkeIntuitionisticSemantics L MD M SM} {usSM: UpwardsSemantics L MD M SM} {UsSM: UnitarySemantics L MD M SM} : @UnitarySemantics L _ _ _ _ MD _ M kiM (DownwardsClosure_SA ) SM kiSM.
 Proof.
   intros m; simpl.
   rewrite <- DownwardsClosure_pre_unit.
@@ -88,7 +88,7 @@ Proof.
       reflexivity.
 Defined.
 
-Definition UsSM {L: Language} {nL: NormalLanguage L} {pL: PropositionalLanguage L} {SL: SeparationLanguage L} {uSL: UnitarySeparationLanguage L} {MD: Model} {kMD: KripkeModel MD} (M: Kmodel) {kiM: KripkeIntuitionisticModel (Kworlds M)} {J: Join  (Kworlds M)} {SA: SeparationAlgebra (Kworlds M)} {uSA: UpwardsClosedSeparationAlgebra (Kworlds M)} {USA: UnitarySeparationAlgebra (Kworlds M)} {SM: Semantics L MD} {kiSM: KripkeIntuitionisticSemantics L MD M SM} {usSM: UpwardsSemantics L MD M SM} {UsSM: UnitarySemantics L MD M SM} : @UnitarySemantics L _ _ _ _ MD _ M kiM (DownwardsClosure_SA ) (DownwardsClosure_USA) SM kiSM.
+Definition UsSM {L: Language} {nL: NormalLanguage L} {pL: PropositionalLanguage L} {SL: SeparationLanguage L} {uSL: UnitarySeparationLanguage L} {MD: Model} {kMD: KripkeModel MD} (M: Kmodel) {kiM: KripkeIntuitionisticModel (Kworlds M)} {J: Join  (Kworlds M)} {SA: SeparationAlgebra (Kworlds M)} {uSA: UpwardsClosedSeparationAlgebra (Kworlds M)} {USA: UnitarySeparationAlgebra (Kworlds M)} {SM: Semantics L MD} {kiSM: KripkeIntuitionisticSemantics L MD M SM} {usSM: UpwardsSemantics L MD M SM} {UsSM: UnitarySemantics L MD M SM} : @UnitarySemantics L _ _ _ _ MD _ M kiM (DownwardsClosure_SA ) SM kiSM.
 Proof.
   intros m; simpl.
   rewrite <- DownwardsClosure_pre_unit.
