SeparationLogic/SoundCompleteParameter.v
@@ -1,0 +1,24 @@
+Record SL_Parameter: Type := {
+  EM: bool;
+  IC: bool;
+  WEM: bool;
+  SCE: bool;
+  EMP: bool
+}.
+
+Record SA_Parameter: Type := {
+  ID: bool;
+  NB: bool;
+  BJ: bool;
+  GC: bool;
+  Uni: bool
+}.
+
+Inductive Parameter_coincide (SLP: SL_Parameter) (SAP: SA_Parameter) : Prop :=
+  Build_Parameter_coincide:
+    EM SLP = ID SAP ->
+    IC SLP = NB SAP ->
+    WEM SLP = BJ SAP ->
+    SCE SLP = GC SAP ->
+    EMP SLP = Uni SAP ->
+    Parameter_coincide SLP SAP.
